template-coq/theories/utils/wGraph.v
@@ -1,8 +1,10 @@
-Require Import Peano_dec Nat Lia ssrbool.
+Require Import ZArith Zcompare Lia ssrbool.
 Require Import MSets.MSetList MSetFacts MSetProperties.
 From MetaCoq.Template Require Import MCUtils.
 
-Lemma fold_max_In n m l (H : fold_left max l n = m)
+Local Open Scope Z_scope.
+
+Lemma fold_max_In n m l (H : fold_left Z.max l n = m)
   : n = m \/ In m l.
 Proof.
   revert n H; induction l; cbn; intros n H.
@@ -11,8 +13,8 @@ Proof.
   apply or_assoc. destruct H; [left|now right]. lia.
 Qed.
 
-Lemma fold_max_le n m l (H : n <= m \/ Exists (Peano.le n) l)
-  : n <= fold_left Nat.max l m.
+Lemma fold_max_le n m l (H : n <= m \/ Exists (Z.le n) l)
+  : n <= fold_left Z.max l m.
 Proof.
   revert m H; induction l; cbn in *; intros m [H|H].
   assumption. inversion H.
@@ -22,7 +24,7 @@ Proof.
 Qed.
 
 Lemma fold_max_le' n m l (H : In n (m :: l))
-  : n <= fold_left Nat.max l m.
+  : n <= fold_left Z.max l m.
 Proof.
   apply fold_max_le. destruct H.
   left; lia. right. apply Exists_exists.
@@ -35,10 +37,10 @@ Qed.
 
 Module Nbar.
   (* None is -∞ *)
-  Definition t := option nat.
+  Definition t := option Z.
   Definition max (n m : t) : t :=
     match n, m with
-    | Some n, Some m => Some (max n m)
+    | Some n, Some m => Some (Z.max n m)
     | Some n, None => Some n
     | None, Some m => Some m
     | _, _ => None
@@ -49,7 +51,7 @@ Module Nbar.
     | _, _ => None
     end.
 
-  Definition S : t -> t := option_map S.
+  Definition S : t -> t := option_map Z.succ.
 
   Definition le (n m : t) : Prop :=
     match n, m with
@@ -136,13 +138,13 @@ Module Nbar.
   Definition add_assoc n m p : n + (m + p) = n + m + p.
   Proof.
     destruct n, m, p; try reflexivity; cbn.
-    now rewrite PeanoNat.Nat.add_assoc.
+    now rewrite Z.add_assoc.
   Defined.
 
   Definition add_0_r n : (n + Some 0 = n)%nbar.
   Proof.
     destruct n; try reflexivity; cbn.
-    now rewrite PeanoNat.Nat.add_0_r.
+    now rewrite Z.add_0_r.
   Defined.
 
   Definition max_lub n m p : n <= p -> m <= p -> max n m <= p.
@@ -153,7 +155,7 @@ Module Nbar.
   Definition add_max_distr_r n m p : max (n + p) (m + p) = max n m + p.
   Proof.
     destruct n, m, p; try reflexivity; cbn.
-    now rewrite PeanoNat.Nat.add_max_distr_r.
+    now rewrite Z.add_max_distr_r.
   Defined.
 
   Definition max_le' n m p : p <= n \/ p <= m -> p <= max n m.
@@ -174,14 +176,14 @@ Module Nbar.
   Definition max_idempotent n : max n n = n.
   Proof.
     destruct n; try reflexivity; cbn.
-    now rewrite PeanoNat.Nat.max_idempotent.
+    now rewrite Z.max_idempotent.
   Defined.
 
   Lemma eq_max n m k (H : max n m = k) : n = k \/ m = k.
   Proof.
-    destruct n, m, k; cbn in H.
-    apply some_inj in H. apply eq_max in H.
-    all: try discriminate; intuition.
+    destruct n, m; simpl in *.
+    destruct (Z.max_spec z z0); intuition congruence.
+    all:intuition.
   Qed.
 
   Lemma fold_max_In n m l (H : fold_left max l n = m)
@@ -217,22 +219,29 @@ Module Nbar.
   Lemma le_dec n m : {n <= m} + {~ n <= m}.
   Proof.
     destruct n as [n|], m as [m|]; cbn.
-    apply Compare_dec.le_dec.
+    simpl. destruct (n ?= m) eqn:comp. left.
+    destruct (Z.compare_spec n m); subst; auto; try lia. discriminate.
+    eapply (proj1 (Z.compare_lt_iff _ _)) in comp. left; lia.
+    eapply (proj1 (Z.compare_gt_iff _ _)) in comp. right; lia.
     all: intuition.
   Defined.
 
   Lemma le_lt_dec n m : ({n <= m} + {m < n})%nbar.
   Proof.
     destruct n as [n|], m as [m|]; cbn.
-    apply Compare_dec.le_lt_dec.
+    simpl. destruct (n ?= m) eqn:comp. left.
+    destruct (Z.compare_spec n m); subst; auto; try lia. discriminate.
+    eapply (proj1 (Z.compare_lt_iff _ _)) in comp. left; lia.
+    eapply (proj1 (Z.compare_gt_iff _ _)) in comp. right; lia.
+
     all: (right; constructor) || (left; constructor).
   Defined.
 
-  Lemma le_plus_r n m : m <= Some n + m.
+  Lemma le_plus_r n m : (0 <= n)%Z -> m <= Some n + m.
   Proof.
     destruct m; cbn; lia.
   Qed.
-
+  
   Lemma le_antisymm {n m} : n <= m -> m <= n -> n = m.
   Proof.
     destruct n, m; cbn; try easy.
@@ -243,13 +252,17 @@ End Nbar.
 
 Import Nbar.
 
+Require Import MSetDecide.
 
 Module WeightedGraph (V : UsualOrderedType).
   Module VSet := MSetList.Make V.
   Module VSetFact := WFactsOn V VSet.
   Module VSetProp := WPropertiesOn V VSet.
+  Module VSetDecide := WDecide (VSet).
+  Ltac sets := VSetDecide.fsetdec.
+
   Module Edge.
-    Definition t := (V.t * nat * V.t)%type.
+    Definition t := (V.t * Z * V.t)%type.
     Definition eq : t -> t -> Prop := eq.
     Definition eq_equiv : RelationClasses.Equivalence eq := _.
 
@@ -275,7 +288,7 @@ Module WeightedGraph (V : UsualOrderedType).
       := fun '(x, n, y) '(x', n', y') => match V.compare x x' with
                                       | Lt => Lt
                                       | Gt => Gt
-                                      | Eq => match PeanoNat.Nat.compare n n' with
+                                      | Eq => match Z.compare n n' with
                                              | Lt => Lt
                                              | Gt => Gt
                                              | Eq => V.compare y y'
@@ -287,7 +300,7 @@ Module WeightedGraph (V : UsualOrderedType).
       pose proof (V.compare_spec x1 x2) as H1.
       destruct (V.compare x1 x2); cbn in *; inversion_clear H1.
       2-3: constructor; intuition.
-      subst. pose proof (PeanoNat.Nat.compare_spec n1 n2) as H2.
+      subst. pose proof (Z.compare_spec n1 n2) as H2.
       destruct (n1 ?= n2); cbn in *; inversion_clear H2.
       2-3: constructor; intuition.
       subst. pose proof (V.compare_spec y1 y2) as H3.
@@ -297,12 +310,13 @@ Module WeightedGraph (V : UsualOrderedType).
 
     Definition eq_dec : forall x y : t, {x = y} + {x <> y}.
       unfold eq. decide equality. apply V.eq_dec.
-      decide equality. apply PeanoNat.Nat.eq_dec. apply V.eq_dec.
+      decide equality. apply Z.eq_dec. apply V.eq_dec.
     Defined.
     Definition eqb : t -> t -> bool := fun x y => match compare x y with
                                           | Eq => true
                                           | _ => false
                                           end.
+    
   End Edge.
   Module EdgeSet:= MSets.MSetList.Make Edge.
   Module EdgeSetFact := WFactsOn Edge EdgeSet.
@@ -316,10 +330,13 @@ Module WeightedGraph (V : UsualOrderedType).
 
   Definition e_source : Edge.t -> V.t := fst ∘ fst.
   Definition e_target : Edge.t -> V.t := snd.
-  Definition e_weight : Edge.t -> nat := snd ∘ fst.
+  Definition e_weight : Edge.t -> Z := snd ∘ fst.
   Notation "x ..s" := (e_source x) (at level 3, format "x '..s'").
   Notation "x ..t" := (e_target x) (at level 3, format "x '..t'").
   Notation "x ..w" := (e_weight x) (at level 3, format "x '..w'").
+
+  Definition opp_edge (e : Edge.t) : Edge.t :=
+    (e..t, - e..w, e..s).
 
   Definition labelling := V.t -> nat.
 
@@ -330,7 +347,8 @@ Module WeightedGraph (V : UsualOrderedType).
       (VSet.add x (V G), (E G), (s G)).
 
     Definition add_edge e : t :=
-      (VSet.add e..s (VSet.add e..t (V G)), EdgeSet.add e (E G), (s G)).
+      (VSet.add e..s (VSet.add e..t (V G)), 
+      EdgeSet.add e (E G), (s G)).
 
     Definition Edges x y := ∑ n, EdgeSet.In (x, n, y) (E G).
 
@@ -361,20 +379,21 @@ Module WeightedGraph (V : UsualOrderedType).
     Fixpoint length {x y} (p : Paths x y) :=
       match p with
       | paths_refl x => 0
-      | paths_step e p => Datatypes.S (length p)
+      | paths_step e p => Z.succ (length p)
       end.
 
     (* Global Instance Paths_refl : CRelationClasses.Reflexive Paths := paths_refl. *)
     (* Global Instance Paths_trans : CRelationClasses.Transitive Paths := @concat. *)
 
-
-    Class invariants := mk_invariant :
-      (* E ⊆ V × V *)
-      (forall e, EdgeSet.In e (E G) -> VSet.In e..s (V G) /\ VSet.In e..t (V G))
-      (* s ∈ V *)
-      /\  VSet.In (s G) (V G)
-      (* s is a source *)
-      /\ (forall x, VSet.In x (V G) -> ∥ Paths (s G) x ∥).
+    Class invariants := mk_invariant
+      { edges_vertices : (* E ⊆ V × V *)
+         (forall e, EdgeSet.In e (E G) -> VSet.In e..s (V G) /\ VSet.In e..t (V G));
+        (* s ∈ V *)
+        source_vertex : VSet.In (s G) (V G);
+        (* s is a source that is lower than any other node *)
+        source_paths : forall x, VSet.In x (V G) -> ∥ ∑ p : Paths (s G) x, ∥ 0 <= weight p ∥ ∥;
+        (* There can be no universe lower than the source: actually no path back to it. *)
+        source_bottom : forall e, EdgeSet.In e (E G) -> e..t <> s G }.
 
     Context {HI : invariants}.
 
@@ -382,7 +401,7 @@ Module WeightedGraph (V : UsualOrderedType).
     Definition PosPaths x y := exists p : Paths x y, weight p > 0.
 
     Class acyclic_no_loop
-      := Build_acyclic_no_loop : forall x (p : Paths x x), weight p = 0.
+      := Build_acyclic_no_loop : forall x (p : Paths x x), weight p <= 0.
 
     Definition acyclic_no_loop' := forall x, ~ (PosPaths x x).
 
@@ -390,20 +409,15 @@ Module WeightedGraph (V : UsualOrderedType).
     Proof.
       unfold acyclic_no_loop, acyclic_no_loop', PosPaths.
       split.
-      - intros H x [p HH]. specialize (H x p); lia.
-      - intros H x p.
-        destruct (PeanoNat.Nat.eq_0_gt_0_cases (weight p));
-          firstorder.
+      - intros H x [p HH]. specialize (H x p). lia.
+      - intros H x p. firstorder.
     Qed.
 
     Definition correct_labelling (l : labelling) :=
-      l (s G) = 0 /\
-      forall e, EdgeSet.In e (E G) -> l e..s + e..w <= l e..t.
+      l (s G) = 0%nat /\
+      forall e, EdgeSet.In e (E G) -> Z.of_nat (l e..s) + e..w <= Z.of_nat (l e..t).
 
-    Definition leq_vertices n x y := forall l, correct_labelling l -> l x + n <= l y.
-
-
-
+    Definition leq_vertices n x y := forall l, correct_labelling l -> Z.of_nat (l x) + n <= Z.of_nat (l y).
 
     Definition DisjointAdd x s s' := VSetProp.Add x s s' /\ ~ VSet.In x s.
 
@@ -434,11 +448,11 @@ Module WeightedGraph (V : UsualOrderedType).
     Proof.
       induction p; cbn; lia.
     Qed.
-
+  
     Fixpoint is_simple {x y} (p : Paths x y) :=
       match p with
       | paths_refl x => true
-      | paths_step e p => negb (VSet.mem x (nodes p)) && is_simple p
+      | @paths_step x y z e p => negb (VSet.mem x (nodes p)) && is_simple p
       end.
 
     Program Definition to_simple : forall {x y} (p : Paths x y),
@@ -605,7 +619,6 @@ Module WeightedGraph (V : UsualOrderedType).
       intros [H _] z Hz. apply H; intuition.
     Qed.
 
-
     Fixpoint snodes {s x y} (p : SimplePaths s x y) : VSet.t :=
       match p with
       | spaths_refl s x => VSet.empty
@@ -613,12 +626,12 @@ Module WeightedGraph (V : UsualOrderedType).
       end.
 
     Definition split {s x y} (p : SimplePaths s x y)
-      : forall u, {VSet.In u (snodes p)} + {u = y}
-             -> SimplePaths (VSet.remove u s) x u * SimplePaths s u y.
+      : forall u, {VSet.In u (snodes p)} + {u = y} -> 
+        SimplePaths (VSet.remove u s) x u * SimplePaths s u y.
     Proof.
       induction p; intros u Hu; cbn in *.
       - induction Hu. eapply False_rect, VSet.empty_spec; eassumption.
-        subst; split; constructor.
+        subst. split; constructor.
       - induction (V.eq_dec x u) as [Hx|Hx].
         + split. subst; constructor.
           econstructor; try eassumption; subst; eassumption.
@@ -642,7 +655,7 @@ Module WeightedGraph (V : UsualOrderedType).
       - simpl. destruct (V.eq_dec x u) as [X|X]; simpl.
         + destruct X; reflexivity.
         + rewrite weight_SimplePaths_sub.
-          rewrite <- PeanoNat.Nat.add_assoc.
+          rewrite <- Z.add_assoc.
           now rewrite IHp.
     Qed.
 
@@ -677,8 +690,15 @@ Module WeightedGraph (V : UsualOrderedType).
       : sweight (split' p).1 + sweight (split' p).2 = sweight p.
     Proof.
       unfold split'; apply weight_split.
-    Defined.
+    Defined.    
 
+    Lemma DisjointAdd_union {s s' s'' x} (H : DisjointAdd x s s')
+      : ~ VSet.In x s'' -> DisjointAdd x (VSet.union s s'') (VSet.union s' s'').
+    Proof.
+      destruct H as [hadd hin].
+      split.
+      now eapply VSetProp.union_Add. sets.
+    Qed.
 
     Lemma DisjointAdd_remove1 {s x} (H : VSet.In x s)
       : DisjointAdd x (VSet.remove x s) s.
@@ -690,6 +710,19 @@ Module WeightedGraph (V : UsualOrderedType).
         + now subst.
         + eapply VSetFact.remove_3; eassumption.
       - now apply VSetFact.remove_1.
+    Qed.
+    
+    Global Instance Add_Proper : Proper (eq ==> VSet.Equal ==> VSet.Equal ==> iff) VSetProp.Add.
+    Proof.
+      intros x y -> s0 s1 eq s0' s1' eq'.
+      unfold VSetProp.Add. now setoid_rewrite eq; setoid_rewrite eq'.
+    Qed.
+
+    Global Instance DisjointAdd_Proper : Proper (eq ==> VSet.Equal ==> VSet.Equal ==> iff) DisjointAdd.
+    Proof.
+      intros x y -> s0 s1 eq s0' s1' eq'.
+      unfold DisjointAdd.
+      now rewrite eq, eq'.
     Qed.
 
     Lemma Add_In {s x} (H : VSet.In x s)
@@ -800,9 +833,33 @@ Module WeightedGraph (V : UsualOrderedType).
     (*     + eapply IHq. rewrite weight_add_end. *)
     (*       lia. *)
     (* Qed. *)
+(*     
+    Lemma weight_simplify {s x y} q (p : SimplePaths s x y)
+      : forall {s'} Hs, (0 < weight q /\ 0 <= sweight p) \/ 0 < sweight p ->
+       0 < sweight (simplify q p (s':=s') Hs).π2.
+    Proof.
+      revert s p; induction q.
+      - cbn; intros. intuition. now rewrite weight_SimplePaths_sub.
+      - intros s p s' Hs; cbn. simpl.
+        set (F0 := proj2 (VSetFact.not_mem_iff s x)); clearbody F0.
+        set (F1 := @VSetFact.mem_2 s x); clearbody F1.
+        set (F2 := @simplify_aux2 s x); clearbody F2.
+        destruct (VSet.mem x s).
+        + case_eq (split' p); intros p1 p2 Hp.
+          case_eq (0 <? sweight p2); intro eq.
+          * cbn. apply Z.ltb_lt in eq.
+            rewrite weight_SimplePaths_sub. auto.
+          * intros Hq. eapply IHq. rewrite weight_add_end.
+            pose proof (weight_split' p) as X; rewrite Hp in X; cbn in X.
+            apply Z.ltb_ge in eq.
+            destruct Hq as [[wq wp]|swp].
+            destruct (Z.ltb_spec 0 (weight q)). left; split; auto.
+            all:admit. 
+        + intros w eapply IHq. rewrite weight_add_end. admit.
+    Admitted. *)
 
     Lemma weight_simplify {s x y} q (p : SimplePaths s x y)
-      : forall {s'} Hs, 0 < weight q \/ 0 < sweight p
+      : forall {s'} Hs, (0 < weight q + sweight p)
         -> 0 < sweight (simplify q p (s':=s') Hs).π2.
     Proof.
       revert s p; induction q.
@@ -814,17 +871,15 @@ Module WeightedGraph (V : UsualOrderedType).
         destruct (VSet.mem x s).
         + case_eq (split' p); intros p1 p2 Hp.
           case_eq (0 <? sweight p2); intro eq.
-          cbn. apply PeanoNat.Nat.leb_le in eq.
-          rewrite weight_SimplePaths_sub; lia.
-          eapply IHq. rewrite weight_add_end.
-          pose proof (weight_split' p) as X; rewrite Hp in X; cbn in X.
-          apply PeanoNat.Nat.ltb_ge in eq. lia.
+          * cbn. apply Z.ltb_lt in eq.
+            rewrite weight_SimplePaths_sub; lia.
+          * eapply IHq. rewrite weight_add_end.
+            pose proof (weight_split' p) as X; rewrite Hp in X; cbn in X.
+            apply Z.ltb_ge in eq. rewrite <- X in H. lia.
         + eapply IHq. rewrite weight_add_end. lia.
     Qed.
 
-
-
-    Definition succs (x : V.t) : list (nat * V.t)
+    Definition succs (x : V.t) : list (Z * V.t)
       := let l := List.filter (fun e => V.eq_dec e..s x) (EdgeSet.elements (E G)) in
          List.map (fun e => (e..w, e..t)) l.
 
@@ -835,7 +890,7 @@ Module WeightedGraph (V : UsualOrderedType).
     Fixpoint lsp00 fuel (s : VSet.t) (x z : V.t) : Nbar.t :=
       let base := if V.eq_dec x z then Some 0 else None in
       match fuel with
-      | 0 => base
+      | 0%nat => base
       | Datatypes.S fuel =>
         match VSet.mem x s with
         | true =>
@@ -988,9 +1043,16 @@ Module WeightedGraph (V : UsualOrderedType).
         apply some_inj in H; subst. unshelve eexists; constructor.
     Qed.
 
+    Lemma lsp0_spec_eq0 {s x} n
+      : lsp0 s x x = Some n -> 0 <= n.
+    Proof.
+      intros lspeq.
+      generalize (lsp0_spec_le (spaths_refl s x)).
+      rewrite lspeq. simpl. auto. 
+    Qed.
 
     Lemma correct_labelling_Paths l (Hl : correct_labelling l)
-      : forall x y (p : Paths x y), l x + weight p <= l y.
+      : forall x y (p : Paths x y), Z.of_nat (l x) + weight p <= Z.of_nat (l y).
     Proof.
       induction p. cbn; lia.
       apply proj2 in Hl.
@@ -998,7 +1060,7 @@ Module WeightedGraph (V : UsualOrderedType).
     Qed.
 
     Lemma correct_labelling_lsp {x y n} (e : lsp x y = Some n) :
-      forall l, correct_labelling l -> l x + n <= l y.
+      forall l, correct_labelling l -> Z.of_nat (l x) + n <= Z.of_nat (l y).
     Proof.
       eapply lsp0_spec_eq in e as [p Hp].
       intros l Hl; eapply correct_labelling_Paths with (p:= to_paths p) in Hl.
@@ -1028,18 +1090,28 @@ Module WeightedGraph (V : UsualOrderedType).
       2: unshelve eapply (lsp0_spec_le (add_end p1 (n; He) _)).
       subst; rewrite weight_add_end; cbn.
       pose proof (sweight_weight p2) as HH.
-      rewrite HG in HH. lia.
+      red in HG. specialize (HG _ (to_paths p2)). lia.
       now apply DisjointAdd_remove1.
     Qed.
 
-    Lemma acyclic_lsp0_xx {HG : acyclic_no_loop} s x
-      : lsp0 s x x = Some 0.
+    Definition is_nonpos n := 
+      match n with
+      | Some z => (z <=? 0)
+      | None => false        
+      end.
+
+    Lemma is_nonpos_spec n : is_nonpos n <~> ∑ z, n = Some z /\ z <= 0.
     Proof.
-      pose proof (lsp0_spec_le (spaths_refl s x)) as H; cbn in H.
-      case_eq (lsp0 s x x); [|intro e; rewrite e in H; cbn in H; lia].
-      intros n Hn. apply lsp0_spec_eq in Hn.
-      destruct Hn as [p Hp]. rewrite sweight_weight, HG in Hp.
-      subst; reflexivity.
+      unfold is_nonpos.
+      split.
+      - destruct n; try intuition congruence.
+        intros le. eapply Z.leb_le in le. exists z; intuition eauto.
+      - intros [z [-> le]]. now eapply Z.leb_le.
+    Qed.
+
+    Lemma is_nonpos_nbar n : is_nonpos n -> (n <= Some 0)%nbar.
+    Proof.
+      now intros [z [-> le]]%is_nonpos_spec.
     Qed.
 
     Definition lsp0_sub {s s' x y}
@@ -1100,7 +1172,7 @@ Module WeightedGraph (V : UsualOrderedType).
     Opaque split reduce SimplePaths_sub.
 
     Lemma weight_simplify2 {HG : acyclic_no_loop} {x z} (p : Paths x z)
-      : sweight (simplify2 p) = weight p.
+      : weight p <= sweight (simplify2 p).
     Proof.
       induction p.
       - reflexivity.
@@ -1113,9 +1185,10 @@ Module WeightedGraph (V : UsualOrderedType).
                x (left (F0 (eq_refl))).
           set (q := split (simplify2 p) x (left (F0 (eq_refl)))) in *.
           destruct q as [q1 q2]; cbn in *.
-          assert (sweight q1 + e.π1 = 0); [|lia].
+          assert (sweight q1 + e.π1 <= 0); [|].
           specialize (HG _ (paths_step e (to_paths q1))). cbn in HG.
-          rewrite <- sweight_weight in HG; lia.
+          rewrite <- sweight_weight in HG. lia.
+          transitivity (e.π1 + sweight (simplify2 p)); [|lia]. rewrite <- H. lia.
         + rewrite weight_SimplePaths_sub. cbn.
           rewrite weight_reduce; intuition.
     Qed.
@@ -1126,8 +1199,7 @@ Module WeightedGraph (V : UsualOrderedType).
       induction p; cbn.
       apply VSetProp.subset_empty.
       apply VSetProp.subset_add_3; [|assumption].
-      apply proj1 in HI.
-      specialize (HI _ e.π2); cbn in HI; apply HI.
+      apply (edges_vertices _ e.π2).
     Qed.
 
     Definition simplify2' {x z} (p : Paths x z) :  SimplePaths (V G) x z.
@@ -1137,39 +1209,106 @@ Module WeightedGraph (V : UsualOrderedType).
     Defined.
 
     Lemma weight_simplify2' {HG : acyclic_no_loop} {x z} (p : Paths x z)
-      : sweight (simplify2' p) = weight p.
+      : weight p <= sweight (simplify2' p).
     Proof.
       unfold simplify2'.
-      now unshelve erewrite weight_SimplePaths_sub, weight_simplify2.
+      unshelve erewrite weight_SimplePaths_sub.
+      eapply weight_simplify2.
     Qed.
 
-
-    Lemma lsp_s x (Hx : VSet.In x (V G))
-      : exists n, lsp (s G) x = Some n.
+    Lemma lsp_s {HG : acyclic_no_loop} x (Hx : VSet.In x (V G))
+      : exists n, lsp (s G) x = Some n /\ 0 <= n.
     Proof.
       case_eq (lsp (s G) x).
-      - intros n H; eexists; reflexivity.
+      - intros n H; eexists; split; [reflexivity|].
+        destruct (source_paths _ Hx) as [[p [w]]].
+        pose proof (lsp0_spec_le (simplify2' p)).
+        unfold lsp in H. rewrite H in H0.
+        simpl in H0.
+        transitivity (weight p); auto.
+        etransitivity; eauto. eapply weight_simplify2'.
       - intro e.
-        destruct (proj2 (proj2 HI) x Hx) as [p].
+        destruct (source_paths x Hx) as [[p [w]]].
         pose proof (lsp0_spec_le (simplify2' p)) as X.
         unfold lsp in e; rewrite e in X. inversion X.
     Qed.
 
+    Lemma Paths_to_source {x} (p : Paths x (s G)) : x = s G /\ weight p = 0.
+    Proof.
+      remember (s G) as source eqn:eq.
+      revert eq. induction p. intros ->; simpl; auto.
+      intros ->.
+      destruct (IHp eq_refl) as [-> w].
+      destruct e as [we ine].
+      specialize (source_bottom _ ine). simpl. congruence.
+    Qed.
+    
+    Lemma lsp_to_s {HG : acyclic_no_loop} {x} (Hx : VSet.In x (V G)) {n}
+      : lsp x (s G) = Some n -> n = 0.
+    Proof.
+      case_eq (lsp x (s G)).
+      - intros z H [= <-].
+        destruct (lsp0_spec_eq _ H).
+        destruct (Paths_to_source (to_paths x0)).
+        rewrite <- sweight_weight in H2. congruence.
+      - intro e. discriminate.
+    Qed.
 
+    Lemma acyclic_lsp0_xx {HG : acyclic_no_loop} s x
+      : lsp0 s x x = Some 0.
+    Proof.
+      pose proof (lsp0_spec_le (spaths_refl s x)) as H; cbn in H.
+      case_eq (lsp0 s x x); [|intro e; rewrite e in H; cbn in H; lia].
+      intros n Hn.
+      pose proof (lsp0_spec_eq0 _ Hn).
+      apply lsp0_spec_eq in Hn.
+      destruct Hn as [p Hp]. rewrite sweight_weight in Hp.
+      red in HG.
+      specialize (HG _ (to_paths p)). subst n. f_equal. lia.
+    Qed.
+
+    (* We don't care about the default value here: lsp is defined everywhere starting from the source. *)
+    Definition to_label (z : option Z) :=
+      match z with
+      | Some (Zpos p) => Pos.to_nat p
+      | _ => 0%nat
+      end.
+
+    Lemma Z_of_to_label (z : Z) : 
+      Z.of_nat (to_label (Some z)) = if 0 <=? z then z else 0.
+    Proof.
+      simpl. destruct z; auto. simpl.
+      apply Z_of_pos_alt.
+    Qed.
+
+    Lemma Z_of_to_label_s {HG : acyclic_no_loop} x : 
+      VSet.In x (V G) ->
+      exists n, lsp (s G) x = Some n /\ 
+        0 <= n /\ (Z.of_nat (to_label (lsp (s G) x))) = n.
+    Proof.
+      intros inx.
+      destruct (lsp_s x inx) as [m [Hm Hpos]].
+      rewrite Hm. eexists; split; auto. split; auto.
+      rewrite Z_of_to_label.
+      eapply Z.leb_le in Hpos. now rewrite Hpos.
+    Qed.
+    
     Lemma lsp_correctness {HG : acyclic_no_loop} :
-        correct_labelling (fun x => option_get 0 (lsp (s G) x)).
+        correct_labelling (fun x => to_label (lsp (s G) x)).
     Proof.
       split.
-      - unfold lsp. now unshelve erewrite acyclic_lsp0_xx.
-      - intros [[x n] y] He; cbn. unfold lsp.
+      - unfold lsp. now rewrite acyclic_lsp0_xx.
+      - intros [[x n] y] He; cbn.
         simple refine (let H := lsp0_triangle_inequality
                                   (V G) (s G) x y n He _
                        in _); [|clearbody H].
-        apply proj1 in HI. specialize (HI _ He); cbn in HI; intuition.
-        destruct (lsp_s x) as [m Hm].
-        + apply proj1 in HI. apply (HI _ He).
-        + unfold lsp in Hm; rewrite Hm in *; cbn in *.
-        destruct (lsp0 (V G) (s G) y); cbn in *; intuition.
+        apply (edges_vertices _ He).
+        fold lsp in H. revert H.
+        destruct (Z_of_to_label_s x) as [xl [eq [pos ->]]]; rewrite ?eq.
+        + apply (edges_vertices _ He).
+        + destruct (Z_of_to_label_s y) as [yl [eq' [ylpos ->]]]; rewrite ?eq'.
+          * apply (edges_vertices _ He).
+          * now simpl.
     Qed.
 
     Lemma SimplePaths_In {s x y} (p : SimplePaths s x y)
@@ -1188,17 +1327,19 @@ Module WeightedGraph (V : UsualOrderedType).
       destruct (lsp0_spec_eq _ Hm) as [p2 Hp2].
       pose proof (lsp0_spec_le (simplify2' (concat (to_paths p1) (to_paths p2))))
         as XX.
-      unshelve erewrite weight_simplify2', weight_concat, <- !sweight_weight in XX ;
+      epose proof (weight_simplify2' (concat (to_paths p1) (to_paths p2))).
+      unshelve erewrite weight_concat, <- !sweight_weight in H;
         try assumption.
-      cbn in XX; erewrite Hp1, Hp2 in XX. exact XX.
+      cbn in H; erewrite Hp1, Hp2 in H.
+      simpl. etransitivity; eauto. simpl. eauto.
     Qed.
 
     Lemma lsp_xx_acyclic
       : VSet.For_all (fun x => lsp x x = Some 0) (V G) -> acyclic_no_loop'.
     Proof.
-      intros H. intros x [p Hp].
+      intros H. intros x [p Hp]. assert (hw: 0 < weight p + sweight ((spaths_refl (V G) x))) by (simpl; lia).
       simple refine (let Hq := weight_simplify p (spaths_refl (V G) _)
-                                               _ (or_introl Hp)
+                                               _ hw
                      in _).
       + exact (V G).
       + etransitivity. apply VSetProp.union_sym.
@@ -1210,10 +1351,9 @@ Module WeightedGraph (V : UsualOrderedType).
         destruct q as [x' q]; cbn in Hq.
         assert (Some (sweight q) <= Some 0)%nbar. {
           erewrite <- H. eapply lsp0_spec_le.
-          eapply SimplePaths_In; eassumption. }
+          eapply (SimplePaths_In q). lia. }
         cbn in H0; lia.
     Defined.
-
 
     Lemma VSet_Forall_reflect P f (Hf : forall x, reflect (P x) (f x)) s
       : reflect (VSet.For_all P s) (VSet.for_all f s).
@@ -1244,7 +1384,7 @@ Module WeightedGraph (V : UsualOrderedType).
       : acyclic_no_loop <-> exists l, correct_labelling l.
     Proof.
       split.
-      intro HG; eexists. now unshelve eapply lsp_correctness.
+      intro HG; eexists. eapply (lsp_correctness).
       intros [l Hl]; eapply acyclic_labelling; eassumption.
     Defined.
 
@@ -1252,9 +1392,9 @@ Module WeightedGraph (V : UsualOrderedType).
       acyclic_no_loop <-> (VSet.For_all (fun x => lsp x x = Some 0) (V G)).
     Proof.
       split.
-      - intros HG x Hx. now unshelve eapply acyclic_lsp0_xx.
+      - intros HG x Hx. unshelve eapply acyclic_lsp0_xx.
       - intros H. apply acyclic_no_loop_loop'.
-        eapply lsp_xx_acyclic; eassumption.
+        now eapply lsp_xx_acyclic.
     Defined.
 
     (* Lemma acyclic_caract3 *)
@@ -1273,7 +1413,8 @@ Module WeightedGraph (V : UsualOrderedType).
       2: now intros x y [].
       apply iff_forall; intro x.
       apply iff_forall; intro Hx.
-      destruct (lsp x x). destruct n. all: split; congruence.
+      split. now intros ->.
+      destruct lsp as [[]|]; try congruence.
     Qed.
 
     (* Lemma is_acyclic_correct : reflect acyclic_no_loop is_acyclic. *)
@@ -1293,16 +1434,21 @@ Module WeightedGraph (V : UsualOrderedType).
     exists k. assumption.
   Defined.
 
-
-
+  Definition add_edges G e :=
+    add_edge (add_edge G e) (opp_edge e).
+  
   Section graph2.
     Context (G : t) {HI : invariants G} {HG : acyclic_no_loop G}.
+    Arguments sweight {G s x y}.
+    Arguments weight {G x y}.
+
 
     Section subgraph.
       Context (y_0 x_0 : V.t) (Vx : VSet.In x_0 (V G))
               (Vy : VSet.In y_0 (V G))
               (Hxs : lsp G x_0 y_0 = None)
-              (K : nat).
+              (x_0ns : x_0 <> s G)
+              (K : Z).
 
       Local Definition G' : t
         := (V G, EdgeSet.add (y_0, K, x_0) (E G), s G).
@@ -1315,15 +1461,79 @@ Module WeightedGraph (V : UsualOrderedType).
         exists e.π1. cbn. apply EdgeSet.add_spec; right. exact e.π2.
       Defined.
 
+      Lemma to_G'_weight {u v} (p : Paths G u v)
+        : weight (to_G' p) = weight p.
+      Proof.
+        clear.
+        induction p. reflexivity.
+        simpl. now rewrite IHp.
+      Qed.
+
+      Opaque Edge.eq_dec.
+
+
+      Definition from_G'_path {u v} (q : Paths G' u v)
+        : Paths G u v + (Paths G u y_0 * Paths G x_0 v).
+      Proof.
+        clear -q. induction q.
+        - left; constructor.
+        - induction (Edge.eq_dec (y_0, K, x_0) (x, e.π1, y)) as [XX|XX].
+          + right. split.
+            * rewrite (fst_eq (fst_eq XX)); constructor.
+            * destruct IHq as [IHq|IHq].
+              -- now rewrite (snd_eq XX).
+              -- exact IHq.2.
+          + induction IHq as [IHq|IHq].
+            * left. econstructor; try eassumption.
+              exists e.π1. exact (EdgeSetFact.add_3 XX e.π2).
+            * right. split.
+              -- econstructor; try eassumption.
+                 2: exact IHq.1.
+                 exists e.π1. exact (EdgeSetFact.add_3 XX e.π2).
+              -- exact IHq.2.
+      Defined.
+
+
+      Lemma from_G'_path_weight {u v} (q : Paths G' u v)
+        : weight q = match from_G'_path q with
+                    | inl q' => weight q'
+                    | inr (q1, q2) => weight q1 + K + weight q2
+                      end.
+      Proof.
+        clear -HI HG Hxs.
+        induction q.
+        - reflexivity.
+        - simpl.
+          destruct (Edge.eq_dec (y_0, K, x_0) (x, e.π1, y)) as [XX|XX]; simpl.
+          + destruct (fst_eq (fst_eq XX)). simpl.
+            inversion XX. 
+            destruct (from_G'_path q) as [q'|[q1 q2]]; simpl.
+            * destruct (snd_eq XX); cbn.
+              destruct e as [e He]; cbn in *. lia.
+            * subst y. rewrite IHq.
+              simple refine (let XX := lsp0_spec_le
+                                         G (simplify2' G q1) in _).
+              unfold lsp in *. rewrite Hxs in XX; inversion XX.
+          + destruct (from_G'_path q) as [q'|[q1 q2]]; simpl.
+            * lia.
+            * lia.
+      Qed.
+
       Global Instance HI' : invariants G'.
       Proof.
         split.
         - cbn. intros e He. apply EdgeSet.add_spec in He; destruct He as [He|He].
           subst; cbn. split; assumption.
           now apply HI.
-        - split. apply HI.
-          intros z Hz. pose proof (HI.p2.p2 z Hz).
-          sq; now apply to_G'.
+        - apply HI.
+        - intros z Hz. epose proof (source_paths G z Hz).
+          destruct H as [[p [w]]]. sq. exists (to_G' p).
+          sq. now rewrite to_G'_weight.
+        - intros z Hz.
+          unfold G' in Hz.
+          eapply EdgeSet.add_spec in Hz as [->|ine].
+          now simpl.
+          apply (source_bottom G _ ine).
       Qed.
 
       Definition from_G' {S u v} (q : SimplePaths G' S u v)
@@ -1349,9 +1559,6 @@ Module WeightedGraph (V : UsualOrderedType).
               -- eapply SimplePaths_sub; [|exact IHq.2].
                  eapply DisjointAdd_Subset; eassumption.
       Defined.
-
-      Arguments sweight {G s x y}.
-      Opaque Edge.eq_dec.
 
       Lemma from_G'_weight {S u v} (q : SimplePaths G' S u v)
         : sweight q = match from_G' q with
@@ -1384,17 +1591,18 @@ Module WeightedGraph (V : UsualOrderedType).
         apply acyclic_caract2. exact _. intros x Hx.
         pose proof (lsp0_spec_le G' (spaths_refl G' (V G') x)) as H; cbn in H.
         case_eq (lsp0 G' (V G) x x); [|intro e; rewrite e in H; cbn in H; lia].
-        intros m Hm. unfold lsp; cbn; rewrite Hm.
+        intros m Hm. unfold lsp; cbn; rewrite Hm. rewrite Hm in H.
+        simpl in H.
         apply lsp0_spec_eq in Hm.
         destruct Hm as [p Hp]. subst.
         pose proof (from_G'_weight p) as XX.
         destruct (from_G' p).
-        - f_equal; now rewrite (sweight_weight G s0), HG in XX.
+        - f_equal. rewrite (sweight_weight G s0) in XX.
+          specialize (HG _ (to_paths G s0)). lia.
         - simple refine (let XX := lsp0_spec_le
             G (simplify2' G (concat G (to_paths G p0.2) (to_paths G p0.1))) in _).
           unfold lsp in *; rewrite Hxs in XX; inversion XX.
       Qed.
-
 
       Lemma lsp_G'_yx : (Some K <= lsp G' y_0 x_0)%nbar.
       Proof.
@@ -1411,7 +1619,7 @@ Module WeightedGraph (V : UsualOrderedType).
       Qed.
 
       Lemma correct_labelling_lsp_G'
-        : correct_labelling G (option_get 0 ∘ lsp G' (s G')).
+        : correct_labelling G (to_label ∘ (lsp G' (s G'))).
       Proof.
         pose proof (lsp_correctness G') as XX.
         split. exact XX.p1.
@@ -1459,7 +1667,9 @@ Module WeightedGraph (V : UsualOrderedType).
           + apply max_le'. left. apply lsp0_spec_le.
           + apply max_le'. right.
             apply (plus_le_compat (Some (sweight p1 + K)) _ (Some (sweight p2))).
-            * cbn. now rewrite sweight_weight, HG.
+            * cbn. rewrite sweight_weight.
+              specialize (HG _ (to_paths G p1)). simpl in *.
+              assert (forall x n, n <= 0 -> n + x <= x). lia. apply H. auto.
             * apply lsp0_spec_le.
         - apply max_lub. apply lsp_G'_incr.
           case_eq (lsp G x_0 x); cbn; [intros k Hk|trivial].
@@ -1490,6 +1700,302 @@ Module WeightedGraph (V : UsualOrderedType).
     End subgraph.
 
 
+    Lemma VSet_add_remove x y p : 
+      x <> y ->
+      VSet.Equal (VSet.add x (VSet.remove y p)) (VSet.remove y (VSet.add x p)).
+    Proof. now sets. Qed.
+    
+    Lemma VSet_remove_add x p : 
+      ~ VSet.In x p ->
+      VSet.Equal (VSet.remove x (VSet.add x p)) p.
+    Proof. now sets. Qed.
+
+
+    Lemma VSet_add_add x y p : 
+      VSet.Equal (VSet.add x (VSet.add y p)) (VSet.add y (VSet.add x p)).
+    Proof. now sets. Qed.
+
+    Lemma VSet_add_add_same x p : 
+      VSet.Equal (VSet.add x (VSet.add x p)) (VSet.add x p).
+    Proof. now sets. Qed.
+
+    Lemma SimplePaths_sets {s x y} (p : SimplePaths G s x y)
+      : x = y \/ VSet.In x s.
+    Proof.
+      induction p. left; auto.
+      destruct IHp; subst. right.
+      destruct d.
+      apply H. left; auto.
+      right. apply d. left; auto.
+    Qed.
+
+    Arguments paths_refl {G x}.
+    Arguments paths_step {G x y z}.
+    
+    Fixpoint Paths_add_end {x y z} (p : Paths G x y) : Edges G y z -> Paths G x z :=
+      match p with
+      | paths_refl => fun e => paths_step e paths_refl
+      | paths_step e' p' => fun e => paths_step e' (Paths_add_end p' e)
+      end.
+
+    Lemma Paths_add_end_weight {x y z} (p : Paths G x y) (e : Edges G y z) : weight (Paths_add_end p e) = weight p + e.π1.
+    Proof.
+      induction p; simpl; auto. lia.
+      rewrite IHp. lia.
+    Qed.
+  
+    Require Import ssreflect.
+
+    Lemma negbe {b} : ~~ b <-> (~ b).
+    Proof.
+      intuition try congruence.
+      now rewrite H0 in H.
+      now destruct b.
+    Qed.
+
+    Lemma In_nodes_app_end {x y z} (p : Paths G x y) (e : Edges G y z) i : 
+      VSet.In i (nodes G (Paths_add_end p e)) -> 
+      VSet.In i (nodes G p) \/ i = y.
+    Proof.
+      induction p; simpl; try sets.
+      rewrite VSet.add_spec.
+      intros []; subst.
+      - sets.
+      - specialize (IHp _ H). sets.
+    Qed.
+
+    Lemma paths_add_end_simpl {x y z} (p : Paths G x y) (e : Edges G y z) : 
+      is_simple _ p -> ~~ VSet.mem y (nodes G p) -> is_simple _ (Paths_add_end p e).
+    Proof.
+      induction p; simpl; auto.
+      move/andP => [nmen iss].
+      specialize (IHp e iss). intros Hm%negbe.
+      rewrite andb_and. split; auto.
+      apply negbe. intro. 
+      apply VSet.mem_spec in H.
+      apply Hm. eapply In_nodes_app_end in H as [inn | ->].
+      eapply negbe in nmen. now elim nmen; apply VSet.mem_spec.
+      apply VSet.mem_spec. sets.
+      eapply IHp. apply negbe => nmem. eapply VSet.mem_spec in nmem.
+      eapply Hm. eapply VSet.mem_spec, VSet.add_spec. sets.
+    Qed.
+     
+    
+    Definition is_refl {x y} (p : Paths G x y) :=
+        match p with
+        | paths_refl => true
+        | _ => false
+        end.
+
+    Lemma Paths_In {x y} (p : Paths G x y) : 
+      VSet.In x (nodes G p) \/ (x = y /\ is_refl p).
+    Proof.
+      induction p; simpl; auto.
+      sets.
+    Qed.
+
+
+    Definition is_srefl {x y s} (p : SimplePaths G s x y) :=
+        match p with
+        | spaths_refl _ _ _ => true
+        | _ => false
+        end.
+
+
+
+    Definition Disjoint s s' := 
+      VSet.Empty (VSet.inter s s').
+ 
+    Lemma Disjoint_DisjointAdd x s s' s'' : 
+      DisjointAdd x s s' -> 
+      Disjoint s' s'' ->
+      Disjoint s s''.
+    Proof.
+      intros da; unfold Disjoint.
+      intros disj i. specialize (disj i).
+      intros ininter; apply disj.
+      eapply DisjointAdd_Subset in da.
+      sets.
+    Qed.
+      
+
+
+    Program Fixpoint sconcat {s s' x y z} (p : SimplePaths G s x y) : Disjoint s s' -> 
+      SimplePaths G s' y z -> SimplePaths G (VSet.union s s') x z :=
+      match p in SimplePaths _ s x y return Disjoint s s' -> SimplePaths G s' y z -> SimplePaths G (VSet.union s s') x z  with
+      | spaths_refl _ _ _ => fun hin q => SimplePaths_sub _ _ q
+      | @spaths_step _ s s0 x y z' da e p => fun hin q =>
+        @spaths_step _ (VSet.union s s') _ x y z _ e (@sconcat _ _ _ _ _ p _ q)
+      end.
+      Next Obligation. sets. Qed.
+      Next Obligation. 
+      Proof.
+        eapply DisjointAdd_union; eauto.
+        destruct da. unfold Disjoint in hin.
+        intros inxs'. apply (hin x).
+        destruct (H x). specialize (H2 (or_introl eq_refl)).
+        now eapply VSet.inter_spec.
+      Qed.
+      Next Obligation.
+        eapply Disjoint_DisjointAdd in hin; eauto.
+        do 2 red in hin. now specialize (hin a).
+      Qed.
+      
+
+    Fixpoint snodes_sym {s x y} (p : SimplePaths G s x y) : VSet.t :=
+      match p with
+      | @spaths_refl _ _ _ => VSet.empty
+      | @spaths_step _ _ _ x y z H e p => VSet.add y (snodes_sym p)
+      end.
+
+    Lemma snodes_sym_in {s x y} (p : SimplePaths G s x y) : ~ VSet.In x (snodes_sym p).
+    Proof.
+      induction p; simpl; auto. sets.
+    Abort.
+
+    Lemma DisjointAdd_sp {x y s} :
+      forall (p : SimplePaths G s x y),
+      forall z, ~ VSet.In z s ->
+      ((y = z) + ~ VSet.In z (snodes_sym p)).
+    Proof.
+      induction p; simpl. right; sets.
+      intros z' hin.
+      specialize (IHp z').
+      forward IHp.
+      eapply DisjointAdd_Subset in d.
+      intro; apply hin; now eapply d.
+      destruct IHp as [|]. left; auto.
+      auto.
+      destruct (V.eq_dec z z'); auto. subst.
+      right.
+      intros hin'.
+      eapply VSet.add_spec in hin'. destruct hin'. subst.
+      destruct (SimplePaths_sets p); auto.
+      eapply DisjointAdd_Subset in d.
+      now apply hin, d.
+      contradiction. 
+    Qed.
+
+    Lemma DisjointAdd_remove_add {x s} :
+      DisjointAdd x (VSet.remove x s) (VSet.add x s).
+    Proof. split; [intro|]; sets. Qed.
+
+    Lemma DisjointAdd_Equal x s s' s'' : DisjointAdd x s s' -> VSet.Equal s' s'' -> DisjointAdd x s s''.
+    Proof. now intros d <-. Qed.
+
+    Lemma DisjointAdd_Equal_l x s s' s'' : DisjointAdd x s s' -> VSet.Equal s s'' -> DisjointAdd x s'' s'.
+    Proof. now intros d <-. Qed.
+
+    Lemma DisjointAdd_remove_inv {x s s' z} : DisjointAdd x s (VSet.remove z s') -> 
+      VSet.Equal s (VSet.remove z s).
+    Proof.
+      intros [].
+      intros i. rewrite VSet.remove_spec.
+      intuition auto. subst.
+      specialize (proj2 (H z) (or_intror H1)).
+      rewrite VSet.remove_spec.
+      intuition.
+    Qed.
+
+    (* x + 1 <= y
+      y -1 <= x ->  x = x, y = y, x <= y - 1 <= x -> x = y - 1
+
+      x + 1 <= y
+      y - 2 <= x -> x -1 <= x -> trivial.
+      
+      x <= y - 1
+      
+      y - 1 <= x + 1 -> y <= x + 2 <= y + 1 <= ....
+      
+      <= y - 2 -> y - 1 
+      
+      y - -2 -> x - + 1 - y => y - 1 <= y
+      
+      <= y - 2 
+    *)
+
+    Lemma reflexive_spaths_weight {s x} (P : SimplePaths G s x x) : sweight _ P <= 0.
+    Proof.
+      specialize (HG _ (to_paths G P)).
+      move: HG.
+      now rewrite sweight_weight.
+    Qed.
+
+    (*
+    Definition SimplePaths_sym_aux_gen {x y s s'} (p : SimplePaths G s' x y) : 
+      VSet.Equal s' (VSet.remove y s) ->
+      SimplePaths G (VSet.remove x (snodes_sym p)) y x * 
+      SimplePaths G (VSet.add y (snodes_sym p)) x x.
+    Proof.
+      induction p in s |- *; simpl.
+      intros. split; exact (spaths_refl _ _ x).
+      set oppe : Edges G y x := (edge_opp e).
+      intros Hs'.
+      eapply DisjointAdd_Equal in d; eauto.
+      specialize (IHp _ (DisjointAdd_remove_inv d)) as [IHp IH'].
+      unshelve eset (add_end := add_end (s' :=VSet.add y (snodes_sym p)) G IHp oppe _).
+      eapply DisjointAdd_remove_add.
+      destruct (split' G add_end).
+      split.
+      2:{ eapply SimplePaths_sub; eauto. abstract sets. }
+      exact s1.
+    Defined.   *)   
+
+    (* Definition SimplePaths_sym_aux_gen {x y s s'} (p : SimplePaths G s' x y) : 
+      VSet.Equal s' (VSet.remove y s) ->
+      SimplePaths G (snodes_sym p) y x * ~ VSet.In x (snodes_sym p).
+    Proof.
+      induction p in s |- *; simpl.
+      intros. split. exact (spaths_refl _ _ x). sets.
+      epose proof (proj1 (proj2 HI) _ e.π2).
+      set oppe : Edges G y x := (-e.π1; H).
+      intros Hs'.
+      eapply DisjointAdd_Equal in d; eauto.
+      specialize (IHp _ (DisjointAdd_remove_inv d)) as [IHp nin].
+      unshelve eset (add_end := add_end (s' :=VSet.add y (snodes_sym p)) G IHp oppe _).
+      now eapply DisjointAdd_add2.
+      split; auto.
+      destruct d.
+      todo String.EmptyString. *)
+(*       
+      intros hin. apply VSet.add_spec in hin.
+      destruct hin; subst. admit.
+      destruct (split' G add_end).
+      epose proof (sconcat s1 _ s2). *)
+    (* Defined. *)
+    
+
+    Lemma Zle_opp {n m} : - n <= m <-> - m <= n.
+    Proof. lia. Qed.
+
+    Lemma Zle_opp' {n m} : n <= m <-> - m <= - n.
+    Proof. lia. Qed.
+
+    (* The two largest simple paths between nodes in both directions bound each other. *)
+    Lemma lsp_sym {x y n} : 
+      lsp G x y = Some n ->
+      (lsp G y x <= Some (-n))%nbar.
+    Proof.
+      intros Hn.        
+      destruct (lsp0_spec_eq _ _ Hn) as [p Hp].
+      destruct (lsp G y x) eqn:lspyx.
+      2:simpl; auto.
+      epose proof (lsp0_spec_eq _ _ lspyx) as [pi Hpi].
+      clear Hn lspyx. rewrite -Hp -Hpi /=.
+      epose proof (weight_simplify G (to_paths _ pi) p (reflexivity _)).
+      destruct simplify as [h loop].
+      simpl in H.
+      move: (HG _ (to_paths _ loop)).
+      rewrite -sweight_weight.
+      rewrite -sweight_weight Hp Hpi in H.
+      rewrite Hp Hpi.
+      destruct (Z.ltb 0 (z + n)) eqn:ltb.
+      eapply Z.ltb_lt in ltb. specialize (H ltb). lia.
+      eapply Z.ltb_nlt in ltb.
+      intros wl.
+      lia.
+    Qed.
+
     Lemma leq_vertices_caract0 {n x y} (Vy : VSet.In y (V G)) :
       leq_vertices G n x y <-> (Some n <= lsp G x y)%nbar.
     Proof.
@@ -1497,9 +2003,9 @@ Module WeightedGraph (V : UsualOrderedType).
       - assert (Vx : VSet.In x (V G)). {
           case_eq (VSet.mem x (V G)); intro Vx; [now apply VSet.mem_spec in Vx|].
           apply False_rect. apply VSetFact.not_mem_iff in Vx.
-          pose (K := Datatypes.S (option_get 0 (lsp G (s G) y))).
+          pose (K := (if (n <=? 0)%Z then (Z.to_nat (Z.of_nat (to_label (lsp G (s G) y)) - n)) + 1 else to_label (lsp G (s G) y))%nat).
           pose (l := fun z => if V.eq_dec z x then K
-                           else option_get 0 (lsp G (s G) z)).
+                           else to_label (lsp G (s G) z)).
           unshelve refine (let XX := Hle l _ in _); subst l K.
           * split.
             -- destruct (V.eq_dec (s G) x).
@@ -1514,17 +2020,61 @@ Module WeightedGraph (V : UsualOrderedType).
           * clearbody XX; cbn in XX.
             destruct (V.eq_dec x x) as [Hx|Hx]; [|now apply Hx].
             destruct (V.eq_dec y x) as [Hy|Hy].
-            now subst. lia. }
-        destruct (lsp_s G y Vy) as [ky Hky].
-        case_eq (lsp G x (s G)).
-        + intros m Hm. etransitivity.
+            now subst.
+            pose proof (lsp_correctness G).
+            specialize (Hle _ H). simpl in Hle.
+            destruct (Z_of_to_label_s G y) as [zl [eq [pos zof]]]; eauto.
+            rewrite zof in XX, Hle.
+            destruct (Z.leb_spec n 0).
+            rewrite Nat2Z.inj_add in XX.
+            rewrite Z2Nat.id in XX; try lia.
+            rewrite zof in XX. lia. }
+        destruct (Z_of_to_label_s G y Vy) as [ly [Hly [Hpos Hlab]]].
+        destruct (Z_of_to_label_s G _ Vx) as [lx [Hlx [poskx Hlab']]].
+        destruct (lsp G x (s G)) eqn:xs.
+        + specialize (Hle _ (lsp_correctness G)) as Hle'; cbn in Hle'.
+          rewrite Hlab Hlab' in Hle'.
+          etransitivity.
           2: exact (lsp_codistance G x (s G) y).
-          rewrite Hm. etransitivity. 2: eapply le_plus_r.
-          specialize (Hle _ (lsp_correctness G)); cbn in Hle.
-          rewrite Hky in *. cbn in *; lia.
-        + intros Hxs.
-          destruct (lsp_s G _ Vx) as [kx Hkx].
-          pose (K := Peano.max kx (Datatypes.S ky)).
+          rewrite xs Hly.
+          assert (n <= ly - lx) by lia.
+          eapply lsp_to_s in xs; eauto.
+          subst z. simpl. lia.
+        + pose (K := Z.max lx (Z.succ ly)).
+          assert (x <> s G). admit.
+          unshelve epose proof (correct_labelling_lsp_G' _ _ _ _ xs H K) as XX;
+            tas; try apply HI.
+          set (G' := G' (s G) x K) in XX.
+          assert (HI' : invariants G'). {
+            eapply HI'; tas. apply HI. }
+          specialize (Hle _ XX); clear XX; cbn in Hle.
+          assert (XX: (Some K <= lsp G' (s G) x)%nbar). {
+            apply lsp_G'_yx. apply HI. }
+          assert (HG' : acyclic_no_loop G'). { apply HG'; eauto. apply HI. }
+          destruct (Z_of_to_label_s G' _ Vx) as [kx' [Hkx' [kx'pos zofx']]].
+          cbn in Hkx'; rewrite Hkx' in XX; cbn in *.
+          rewrite zofx' in Hle.
+          destruct (Z_of_to_label_s G' _ Vy) as [ky' [Hky' [ky'pos zofy']]].
+          cbn in Hky'; rewrite zofy' in Hle; cbn in *.
+          assert (Hle'' : K + n <= ky') by lia; clear Hle.
+          enough ((Some ky' <= Some K + lsp G x y)%nbar) as HH. {
+            revert HH. destruct (lsp G x y); cbn; auto. lia. }
+          unshelve erewrite (lsp_G'_spec_left (s G) x _ xs K) in Hky'. apply HI.
+          apply eq_max in Hky'. destruct Hky' as [Hk|Hk].
+          -- rewrite Hly in Hk. apply some_inj in Hk. subst ky'. simpl. lia.
+          -- rewrite <- H. reflexivity.
+      - case_eq (lsp G x y).
+        * intros m Hm l Hl. rewrite Hm in Hle.
+          apply (lsp0_spec_eq G) in Hm. destruct Hm as [p Hp].
+          pose proof (correct_labelling_Paths G l Hl _ _ (to_paths G p)) as XX.
+          rewrite <- sweight_weight, Hp in XX. cbn in Hle; lia.
+        * intro X; rewrite X in Hle; inversion Hle.
+    Defined.
+
+
+
+
+          pose (K := Z.max lx (Z.succ ly)).
           unshelve epose proof (correct_labelling_lsp_G' _ _ _ _ Hxs K) as XX;
             tas; try apply HI.
           set (G' := G' (s G) x K) in XX.
@@ -1542,8 +2092,11 @@ Module WeightedGraph (V : UsualOrderedType).
             revert HH. destruct (lsp G x y); cbn; lia. }
           unshelve erewrite (lsp_G'_spec_left (s G) x _ Hxs K) in Hky'. apply HI.
           apply eq_max in Hky'. destruct Hky' as [H|H].
-          -- rewrite Hky in H. apply some_inj in H; subst; lia.
-          -- rewrite <- H. reflexivity.
+          -- rewrite Hky in H. apply some_inj in H; subst; try lia.
+             apply lsp_sym in Hkx. rewrite Hxs in Hkx. now simpl in Hkx.
+          -- rewrite <- H. reflexivity. *)
+        eapply lsp_sym in Hkx. destruct (lsp _ x (s G)); try congruence.
+          now simpl in Hkx.
       - case_eq (lsp G x y).
         * intros m Hm l Hl. rewrite Hm in Hle.
           apply (lsp0_spec_eq G) in Hm. destruct Hm as [p Hp].
@@ -1552,6 +2105,24 @@ Module WeightedGraph (V : UsualOrderedType).
         * intro X; rewrite X in Hle; inversion Hle.
     Defined.
 
+    Lemma lsp_vset_in {s x y n} : 
+      lsp0 G s x y = Some n -> 
+      (n = 0 /\ x = y) \/ (VSet.In y (V G)).
+    Proof.
+      intros H.
+      eapply lsp0_spec_eq in H.
+      destruct H. subst n. induction x0.
+      simpl. left; auto. destruct IHx0 as [[sw ->]|IH].
+      destruct e. destruct HI. specialize (H _ i) as [Hs Ht]. right; apply Ht.
+      right; auto.
+    Qed.
+
+
+
+
+    Lemma leq_vertices_caract0 {n x y} (Vy : VSet.In y (V G)) :
+      leq_vertices G n x y <-> (Some n <= lsp G x y)%nbar.
+   
 
     Lemma leq_vertices_caract {n x y} :
       leq_vertices G n x y <-> (if VSet.mem y (V G) then Some n <= lsp G x y
@@ -1651,10 +2222,108 @@ Module WeightedGraph (V : UsualOrderedType).
         apply proj1 in Hl. lia.
     Defined.
 
+    Lemma leq_vertices_caract {n x y} :
+      leq_vertices G n x y <-> (if VSet.mem y (V G) then Some n <= lsp G x y
+                             else (n <= 0)%Z /\ (x = y \/ Some n <= lsp G x (s G)))%nbar.
+    Proof.
+      case_eq (VSet.mem y (V G)); intro Vy;
+        [apply VSet.mem_spec in Vy; now apply leq_vertices_caract0|].
+      split.
+      - intro Hle. apply VSetFact.not_mem_iff in Vy. 
+        assert (nneg : n <= 0).
+        { pose (K := to_label (lsp G (s G) x)).
+          pose (l := fun z => if V.eq_dec z y then K
+                           else to_label (lsp G (s G) z)).
+            unshelve refine (let XX := Hle l _ in _); subst l K.
+            -- split.
+              ++ destruct (V.eq_dec (s G) y).
+                 apply False_rect. apply Vy. subst; apply HI.
+                 now apply lsp_correctness.
+              ++ intros e H.
+                 destruct (V.eq_dec e..s y).
+                 apply False_rect, Vy; subst; now apply HI.
+                 destruct (V.eq_dec e..t y).
+                 apply False_rect, Vy; subst; now apply HI.
+                 now apply lsp_correctness.
+            -- clearbody XX; cbn in XX.
+               destruct (V.eq_dec y y) as [?|?]; simpl in *; [|contradiction].
+               destruct (V.eq_dec x y) as [Hy|Hy]; simpl in *; [intuition|lia]. }
+        split; auto.
+        + destruct (V.eq_dec x y); [now left|right].
+          case_eq (lsp G x (s G)); [intros; cbn; try lia|].
+          eapply lsp_sym in H.
+          pose (l := fun n => if V.eq_dec n y then Z.to_nat z
+            else to_label (lsp G (s G) n)).
+          unshelve refine (let XX := Hle l _ in _); subst l.
+          -- split.
+            ++ destruct (V.eq_dec (s G) y).
+              apply False_rect. apply Vy. subst; apply HI.
+              now apply lsp_correctness.
+            ++ intros e H'.
+              destruct (V.eq_dec e..s y).
+              apply False_rect, Vy; subst; now apply HI.
+              destruct (V.eq_dec e..t y).
+              apply False_rect, Vy; subst; now apply HI.
+              now apply lsp_correctness.
+          -- clearbody XX; cbn in XX.
+            destruct (V.eq_dec y y) as [?|?]; [|contradiction].
+            destruct (V.eq_dec x y) as [Hy|Hy]; simpl in *; [intuition|try lia].
+            destruct (lsp G (s G) x) eqn:elsp.
+            destruct (lsp_vset_in elsp) as [[-> <-]|hin].
+            * simpl in *. lia.
+            * rewrite <-elsp in XX.
+              destruct (Z_of_to_label_s G x hin) as [lz [eq [pos zof]]].
+              rewrite zof in XX. simpl in H. rewrite eq in elsp. injection elsp as ->.
+              lia.
+            * now simpl in H.
+          -- intros Hxs; apply False_rect.
+            case_eq (VSet.mem x (V G)); intro Vx.
+            * apply VSet.mem_spec in Vx.
+              destruct (lsp_s G _ Vx). destruct H.
+              eapply lsp_sym in H. destruct (lsp _ x (s G)); try congruence.
+              now simpl in H.
+            * apply VSetFact.not_mem_iff in Vx.
+              pose (K := option_get 0 (lsp G (s G) x)).
+              pose (l := fun z => if V.eq_dec z y then 0%nat
+                             else if V.eq_dec z x then (Z.to_nat (- n) + 1)%nat
+                             else to_label (lsp G (s G) z)).
+              unshelve refine (let XX := Hle l _ in _); subst l K.
+              --- split.
+               ++ destruct (V.eq_dec (s G) y).
+                  apply False_rect. apply Vy. subst; apply HI.
+                  destruct (V.eq_dec (s G) x).
+                  apply False_rect. apply Vx. subst; apply HI.
+                  now apply lsp_correctness.
+               ++ intros e H.
+                  destruct (V.eq_dec e..s y).
+                  apply False_rect, Vy; subst; now apply HI.
+                  destruct (V.eq_dec e..t y).
+                  apply False_rect, Vy; subst; now apply HI.
+                  destruct (V.eq_dec e..s x).
+                  apply False_rect, Vx; subst; now apply HI.
+                  destruct (V.eq_dec e..t x).
+                  apply False_rect, Vx; subst; now apply HI.
+                  now apply lsp_correctness.
+            --- clearbody XX; cbn in XX.
+               destruct (V.eq_dec y y) as [?|?]; [|contradiction].
+               destruct (V.eq_dec x y) as [Hy|Hy]; simpl in *. contradiction.
+               destruct (V.eq_dec x x) as [?|?]; simpl in *; [lia|contradiction].
+      - intros [e [Hxy|Hxs]] l Hl; subst; [lia|].
+        case_eq (lsp G x (s G)); [|intro H; rewrite H in Hxs; inversion Hxs].
+        intros k Hk.
+        rewrite Hk in Hxs. simpl in Hxs.
+        destruct (lsp0_spec_eq _ _ Hk) as [p Hp].
+        epose proof (correct_labelling_Paths G l Hl _ _ (to_paths G p)).
+        rewrite (proj1 Hl) in H.
+        simpl in Hxs. rewrite <- sweight_weight, Hp in H.
+        transitivity (Z.of_nat (l x) + k). lia.
+        transitivity 0; auto.
+        lia.
+    Qed.
 
-    Definition leqb_vertices n x y : bool :=
-      if VSet.mem y (V G) then le_dec (Some n) (lsp G x y)
-      else Nat.eqb n 0 && (V.eq_dec x y || le_dec (Some 0) (lsp G x (s G))).
+    Definition leqb_vertices z x y : bool :=
+      if VSet.mem y (V G) then if is_left (Nbar.le_dec (Some z) (lsp G x y)) then true else false
+      else (Z.leb z 0 && (V.eq_dec x y || Nbar.le_dec (Some z) (lsp G x (s G))))%bool.
 
     Lemma leqb_vertices_correct n x y
       : leq_vertices G n x y <-> leqb_vertices n x y.
@@ -1665,13 +2334,15 @@ Module WeightedGraph (V : UsualOrderedType).
         discriminate.
       - symmetry; etransitivity. apply andb_and.
         apply Morphisms_Prop.and_iff_morphism.
-        apply PeanoNat.Nat.eqb_eq.
+        apply Z.leb_le.
         etransitivity. apply orb_true_iff.
         apply Morphisms_Prop.or_iff_morphism.
         destruct (V.eq_dec x y); cbn; intuition; try discriminate.
-        destruct (le_dec (Some 0) (lsp G x (s G))); cbn; intuition.
+        destruct (le_dec (Some n) (lsp G x (s G))); cbn; intuition.
         discriminate.
     Qed.
 
   End graph2.
+  
 End WeightedGraph.
+
